add simple record evaluation examples

theories/typing/examples/records.v
@@ -1,12 +1,28 @@
-From iris.proofmode Require Import proofmode.
-From lrust.typing Require Import typing record.
+From iris.program_logic Require Export adequacy weakestpre.
+From iris.algebra Require Import auth.
+From lrust.lang Require Export heap.
+From lrust.lang Require Import proofmode notation.
+From lrust.typing Require Export type.
+From lrust.typing Require Import record int bool.
 From iris.prelude Require Import options.
 
 Section record.
 Context `{!typeGS Σ}.
+Notation iProp := (iProp Σ).
 
-Definition recordv_example := RecordNil.
+Definition re1 := rnil%E.
+Definition re2 := ("i1" /: #1 + #2 :+: "i2" /: #2 :+: rnil)%E.
 Definition record_type := record [("x", int); ("y", int); ("z", bool)].
 
+Example re1_spec: ⊢ WP re1 {{ v, ⌜ v = RecordVNil ⌝ } }.
+Proof.
+rewrite /re1.
+by iApply wp_value.
+Qed.
 
+Example re2_spec: ⊢ WP re2 {{ v,  ⌜ v = ("i1" /: #3 :+: "i2" /: #2 :+: rnil)%V ⌝ }}.
+Proof.
+rewrite /re2.
+by wp_op.
+Qed.
 End record.
